---
tags:
  - Calculus
  - Mathematics
  - derivatives
cssclasses: []
---
# Algebraic Functions

$$
\begin{array}{c}
\dfrac{d}{dx}x^n=nx^{n-1} & \hspace{1.0in} \dfrac{d}{dx}x^{-n}=-nx^{-n-1}
\end{array}
$$

# Trigonometric Functions

$$
\begin{array}{ll}
\dfrac{d}{dx}\sin x=\cos x & \hspace{1.0in} \dfrac{d}{dx}\cos x=-\sin x \\
\dfrac{d}{dx}\tan x=\sec^2x & \hspace{1.0in}  \dfrac{d}{dx}\cot x = -\csc^2x \\
\dfrac{d}{dx}\sec x=\sec x\tan x &\hspace{1.0in} \dfrac{d}{dc}\csc x=-\csc x\cot x 
\end{array}
$$

# Exponential Functions

- [[Euler's constant]] is defined as

$$
e = \lim_{ n \to \infty } \left( 1+\frac{1}{n} \right)^{n}
$$
$$
e = \sum_{n = 0}^{\infty} {\frac{1}{n!}}
$$

- Derivatives of exponential functions are $$
\begin{array}{cc}
\dfrac{d}{dx}e^{x}=e^{x} & \hspace{1in} \dfrac{d}{dx}a^{x}=a^{x}\ln a \\ \dfrac{d}{dx}\ln x=\dfrac{1}{x} & \hspace{1.0in} \dfrac{d}{dc}\log_{a}x=\dfrac{1}{x\ln a}
\end{array}

$$
# Inverse Trigonometric Functions

$$\begin{array}{ll}\displaystyle \frac{d}{{dx}}\left( {{{\sin }^{ - 1}}x} \right) = \frac{1}{{\sqrt {1 - {x^2}} }} & \hspace{1.0in}\displaystyle \frac{d}{{dx}}\left( {{{\cos }^{ - 1}}x} \right) =  - \frac{1}{{\sqrt {1 - {x^2}} }}\\ \displaystyle \frac{d}{{dx}}\left( {{{\tan }^{ - 1}}x} \right) = \frac{1}{{1 + {x^2}}} & \hspace{1.0in}\displaystyle \frac{d}{{dx}}\left( {{{\cot }^{ - 1}}x} \right) =  - \frac{1}{{1 + {x^2}}}\\ \displaystyle \frac{d}{{dx}}\left( {{{\sec }^{ - 1}}x} \right) = \frac{1}{{\left| x \right|\sqrt {{x^2} - 1} }} & \hspace{1.0in}\displaystyle \frac{d}{{dx}}\left( {{{\csc }^{ - 1}}x} \right) =  - \frac{1}{{\left| x \right|\sqrt {{x^2} - 1} }}\end{array}$$
# Hyperbolic Function

- [[Hyperbolic Functions]] are defined as follows
$$

\begin{array}{ll}
\sinh x=\frac{e^{x}-e^{-x}}{2} & \cosh x= \frac{{e^{x}+e^{-x}}}{2}
\end{array}

$$
$$\begin{array}{ll}\displaystyle \frac{d}{{dx}}\left( {\sinh x} \right) = \cosh x & \hspace{1.0in} \displaystyle \frac{d}{{dx}}\left( {\cosh x} \right) = \sinh x\\ \displaystyle \frac{d}{{dx}}\left( {\tanh x} \right) = \mbox{sech}^{2}x & \hspace{1.0in} \displaystyle \frac{d}{{dx}}\left( {\coth x} \right) =  - {\mbox{csch}}^{2}x\\ \displaystyle \frac{d}{{dx}}\left( {{\mbox{sech}}\,x} \right) =  - {\mbox{sech }}x{\mbox{ tanh }}x & \hspace{1.0in} \displaystyle \frac{d}{{dx}}\left( {{\mbox{csch}}\,x} \right) =  - {\mbox{csch }}x{\mbox{ coth }}x\end{array}$$
